@base <http://www.semanticweb.org/labinvirtuo#> .
@prefix liv: <http://www.semanticweb.org/labinvirtuo#> .
@prefix crm: <http://www.cidoc-crm.org/cidoc-crm/> .
@prefix owl: <http://www.w3.org/2002/07/owl#> .
@prefix rdf: <http://www.w3.org/1999/02/22-rdf-syntax-ns#> .
@prefix vann: <http://purl.org/vocab/vann/> .
@prefix dcterms: <http://purl.org/dc/terms/> .
@prefix skos: <http://www.w3.org/2004/02/skos/core#> .
@prefix bibo: <http://purl.org/ontology/bibo/> .
@prefix foaf: <http://xmlns.com/foaf/0.1/> .
@prefix rdfs: <http://www.w3.org/2000/01/rdf-schema#> .
@prefix rico: <https://www.ica.org/standards/RiC/ontology#> . 


#################################################################
#    This file
#################################################################

# This file an overwrite of some properties and somes classes of imported ontologies. 
# These edits are mainly done in order to generate a SHACL file with appropriate restriction (domain / class / cardinality)
# Some new properties / class are created to extend existing ontologies when needed. 

#################################################################
#    This ontology
#################################################################

<http://www.semanticweb.org/labinvirtuo> rdf:type owl:Ontology, bibo:Document ;
  vann:preferredNamespacePrefix "liv";
  vann:preferredNamespaceUri "http://www.semanticweb.org/labinvirtuo/ontologies/2023/0/TTM#";
  dcterms:creator _:node01peopleA ;
  dcterms:contributor "Noé Echard, UTBM", "Cyril Lachèze, UTBM";
  dcterms:title "lab-in-virtuo: A vocabulary for describing history and heritage items" ;
  skos:prefLabel "lab-in-virtuo: A vocabulary for describing history and heritage items" ;
	dcterms:description "lab-in-virtuo: A vocabulary for describing history of techniques and industrial heritage" ;
	# dct:isVersionOf  ;
	# dct:replaces ;
	# vann:example ;
	dcterms:issued "2023-02-27" ;
  # skos:historyNote _:node010722histA  ;
	skos:changeNote _:node010722changA .

_:node01peopleA a foaf:Person ;
  owl:sameAs <https://viaf.org/viaf/1868159234284803371171>;
  foaf:name "Matthieu Quantin" ;
  foaf:workplaceHomepage "https://www.ec-nantes.fr/" .

_:node010722changA rdf:value "describing the onotology itself with vann and others" ;
	dcterms:date "2023-02-27" ;
	dcterms:creator <https://viaf.org/viaf/1868159234284803371171> .


#################################################################
#    Annotation properties
#################################################################

#################################################################
#    Datatypes
#################################################################


#################################################################
#    Data properties
#################################################################


#################################################################
#    Object Properties
#################################################################

liv:otherWallFace rdf:type owl:SymmetricProperty ;#sub class of owl:objectProperty
                     rdfs:domain liv:WallFace ;
                     rdfs:range liv:WallFace ;
                     rdfs:comment """This property associate two faces of tht same wall. This is a symetric property. Note that it is not transitive: example wall A is a façade (outside) it has many otherWallFace inside, one in each room for example. """ ;
                     rdfs:label "other wall face of"@en .



#################################################################
#    Classes
#################################################################

liv:wallFace rdf:type owl:Class ;
                          rdfs:subClassOf crm:E22_Human-Made_Object ;
                          rdfs:comment """This class comprises a wall face, this is the visible face of a wall. The property liv:otherWallFace enables to link one face to the other""" ;
                          rdfs:label "Wall face"@en .

rico:RecordResource rdf:type owl:Class ;
                          rdfs:subClassOf bibo:Document .
